@prefix : <http://lod.tuwien.ac.at/organization/vocab#> .
@prefix dct: <http://purl.org/dc/terms/> .
@prefix org: <http://www.w3.org/ns/org#> .
@prefix owl: <http://www.w3.org/2002/07/owl#> .
@prefix rdf: <http://www.w3.org/1999/02/22-rdf-syntax-ns#> .
@prefix xml: <http://www.w3.org/XML/1998/namespace> .
@prefix xsd: <http://www.w3.org/2001/XMLSchema#> .
@prefix foaf: <http://xmlns.com/foaf/0.1/> .
@prefix rdfs: <http://www.w3.org/2000/01/rdf-schema#> .
@prefix skos: <http://www.w3.org/2004/02/skos/core#> .
@prefix aiiso: <http://purl.org/vocab/aiiso/schema#> .
@base <http://lod.tuwien.ac.at/organization/vocab#> .

<http://lod.tuwien.ac.at/organization/vocab#> rdf:type owl:Ontology ;
                                              
                                              rdfs:label "Vokabular für die Organisationsstruktur von Universitäten"@de ,
                                                         "Vocabulary for the organizational structure of universities"@en ;
                                              
                                              dct:created "2016-02-04"^^xsd:date ;
                                              
                                              dct:modified "2016-02-05"^^xsd:date ;
                                              
                                              dct:abstract "Beschreibt die Domäne der Organisationsstruktur von Universitäten."@de ;
                                              
                                              rdfs:comment "Beschreibt die Domäne der Organisationsstruktur von Universitäten."@de ;
                                              
                                              dct:title "Vokabular für die Organisationsstruktur von Universitäten"@de ;
                                              
                                              rdfs:comment "Describes the domain of the organizational structure of universities."@en ;
                                              
                                              dct:abstract "Describes the domain of the organizational structure of universities."@en ;
                                              
                                              dct:title "Vocabulary for the organizational structure of universities"@en ;
                                              
                                              owl:versionIRI <http://lod.tuwien.ac.at/organization/0.1-SNAPSHOT> ;
                                              
                                              dct:contributor <http://lod.tuwien.ac.at/person/contributor/Kevin_Haller> ;
                                              
                                              owl:imports skos: ,
                                                          org: .


#################################################################
#
#    Object Properties
#
#################################################################


###  http://lod.tuwien.ac.at/organization/vocab#employmentRole

:employmentRole rdf:type owl:ObjectProperty ;
                
                rdfs:label "anstellungsrolle"@de ,
                           "employment role"@en ;
                
                rdfs:comment "Beschreibt welche Anstellunsgrolle (z.B.: Dozent, Tutor) der Agent in der gegebene Mitgliedschaft an einer Universität spielt."@en ,
                             "Indicates the employment role (e.g. tutor, docent, ...) of the agent of a membership in an university."@en ;
                
                rdfs:isDefinedBy <http://lod.tuwien.ac.at/organization/vocab#> ;
                
                rdfs:domain :Employment ;
                
                rdfs:range :EmploymentRole ;
                
                rdfs:subPropertyOf :role .



###  http://lod.tuwien.ac.at/organization/vocab#hasDeanary

:hasDeanary rdf:type owl:FunctionalProperty ,
                     owl:IrreflexiveProperty ,
                     owl:ObjectProperty ;
            
            rdfs:label "hat Dekanat"@de ,
                       "has deanary"@en ;
            
            rdfs:comment "Diese Fakultät hat das gegebene Dekanat. Einer Fakultät kann nur ein Dekanat zugeordnet werden."@de ,
                         "This faculty has the given deanary. A faculty can have only one deanary."@en ;
            
            rdfs:isDefinedBy <http://lod.tuwien.ac.at/organization/vocab#> ;
            
            rdfs:range :Deanery ;
            
            rdfs:subPropertyOf :hasUnit ;
            
            rdfs:domain [ rdf:type owl:Class ;
                          owl:unionOf ( :Department
                                        :Faculty
                                      )
                        ] .



###  http://lod.tuwien.ac.at/organization/vocab#hasInstitute

:hasInstitute rdf:type owl:ObjectProperty ;
              
              rdfs:label "hat Institut"@de ,
                         "has institute"@en ;
              
              rdfs:comment "Diese Fakultät hat das gegebene Institut."@de ,
                           "This faculty has the given institute."@en ;
              
              rdfs:isDefinedBy <http://lod.tuwien.ac.at/organization/vocab#> ;
              
              rdfs:domain :Faculty ;
              
              rdfs:range :Institute ;
              
              rdfs:subPropertyOf :hasUnit .



###  http://lod.tuwien.ac.at/organization/vocab#hasSubOrganization

:hasSubOrganization rdf:type owl:ObjectProperty ;
                    
                    rdfs:label "hat universitäre Suborganisation"@de ,
                               "has university suborganization"@en ;
                    
                    rdfs:isDefinedBy "Die gegebene Universitätsorganisation ist eine Suborganisation dieser Universitätsorganisation."@de ;
                    
                    rdfs:comment "The given university organization is a suborganization of this university organization."@en ;
                    
                    rdfs:isDefinedBy <http://lod.tuwien.ac.at/organization/vocab#> ;
                    
                    rdfs:domain :UniversityOrganization ;
                    
                    rdfs:range :UniversityOrganization ;
                    
                    rdfs:subPropertyOf org:hasSubOrganization .



###  http://lod.tuwien.ac.at/organization/vocab#hasUnit

:hasUnit rdf:type owl:ObjectProperty ;
         
         rdfs:label "hat Organisationseinheit"@de ,
                    "has organizational unit"@en ;
         
         rdfs:commenet "Diese Universitätsorganisation hat die gegebene universitäre Organisationseinheit als Suborganisaiton."@de ,
                       "This university organization has the given university organizational unit as suborganization."@en ;
         
         rdfs:isDefinedBy <http://lod.tuwien.ac.at/organization/vocab#> ;
         
         rdfs:domain :UniversityOrganization ;
         
         rdfs:range :UniversityOrganizationalUnit ;
         
         rdfs:subPropertyOf :hasSubOrganization .



###  http://lod.tuwien.ac.at/organization/vocab#isDeanaryOf

:isDeanaryOf rdf:type owl:FunctionalProperty ,
                      owl:IrreflexiveProperty ,
                      owl:ObjectProperty ;
             
             rdfs:label "ist Dekanat von"@de ,
                        "is deanary of"@en ;
             
             rdfs:comment "Diese Universitätsorganisation ist das Dekanat der gegebenen Fakultät oder Abteilung."@de ,
                          "This university organization is the deanary of the given faculty or division."@en ;
             
             rdfs:isDefinedBy <http://lod.tuwien.ac.at/organization/vocab#> ;
             
             rdfs:domain :Deanery ;
             
             owl:inverseOf :hasDeanary ;
             
             rdfs:subPropertyOf :unitOf ;
             
             rdfs:range [ rdf:type owl:Class ;
                          owl:unionOf ( :Department
                                        :Faculty
                                      )
                        ] .



###  http://lod.tuwien.ac.at/organization/vocab#isInstituteOf

:isInstituteOf rdf:type owl:ObjectProperty ;
               
               rdfs:label "ist Institut von"@de ,
                          "is institute of"@en ;
               
               rdfs:comment "Diese Universitätsorganisation ist ein Institut der gegebenen Universitätsorganisation."@en ,
                            "This university organization is the institute of the given faculty."@en ;
               
               rdfs:isDefinedBy <http://lod.tuwien.ac.at/organization/vocab#> ;
               
               rdfs:range :Faculty ;
               
               rdfs:domain :Institute ;
               
               owl:inverseOf :hasInstitute ;
               
               rdfs:subPropertyOf :unitOf .



###  http://lod.tuwien.ac.at/organization/vocab#role

:role rdf:type owl:ObjectProperty ;
      
      rdfs:label "rolle"@de ,
                 "role"@en ;
      
      rdfs:comment "Beschreibt welche Universitätstrolle (z.B.: Student, Vortragender,...) der Agent in der gegebene Mitgliedschaft an einer Universität spielt."@de ,
                   "Indicates the university role (e.g. student, lecturer, ...) of the agent of a membership in an university."@en ;
      
      rdfs:isDefinedBy <http://lod.tuwien.ac.at/organization/vocab#> ;
      
      rdfs:domain :UniversityMembership ;
      
      rdfs:range :UniversityRole ;
      
      rdfs:subPropertyOf org:role .



###  http://lod.tuwien.ac.at/organization/vocab#subOrganizationOf

:subOrganizationOf rdf:type owl:ObjectProperty ;
                   
                   rdfs:label "ist Suborganisation von"@de ,
                              "is suborganization of"@en ;
                   
                   rdfs:comment "Diese Universitätsorganisation ist eine Suborganisation der gegebenen Universitätsorganisation."@de ,
                                "This university organization is a suborganization of the given organization."@en ;
                   
                   rdfs:isDefinedBy <http://lod.tuwien.ac.at/organization/vocab#> ;
                   
                   rdfs:domain :UniversityOrganization ;
                   
                   rdfs:range :UniversityOrganization ;
                   
                   owl:inverseOf :hasSubOrganization ;
                   
                   rdfs:subPropertyOf org:subOrganizationOf .



###  http://lod.tuwien.ac.at/organization/vocab#unitOf

:unitOf rdf:type owl:ObjectProperty ;
        
        rdfs:label "ist Organisationseinheit von"@de ,
                   "is organizational unit of"@en ;
        
        rdfs:comment "Diese Organisationseinheit einer Universität ist die Einheit einer gegebenen Universitätsorganisation."@de ,
                     "This university organizational unit is the unit of the given university organization."@en ;
        
        rdfs:isDefinedBy <http://lod.tuwien.ac.at/organization/vocab#> ;
        
        rdfs:range :UniversityOrganization ;
        
        rdfs:domain :UniversityOrganizationalUnit ;
        
        owl:inverseOf :hasUnit ;
        
        rdfs:subPropertyOf :subOrganizationOf .





#################################################################
#
#    Classes
#
#################################################################


###  http://lod.tuwien.ac.at/organization/vocab#AcademicLibrary

:AcademicLibrary rdf:type owl:Class ;
                 
                 rdfs:label "Akademische Bibliothek"@de ,
                            "Academic library"@en ;
                 
                 rdfs:subClassOf :UniversityOrganization ,
                                 org:FormalOrganization ;
                 
                 rdfs:comment "Eine akademische Bibliothek ist eine Bibliothek, die einer Universität zugeordnet ist um einerseits die Curricula der Asubildung und andererseits die Forschung von Universitätsorganisationen und Studenten zu unterstützen."@de ,
                              "An academic library is a library that is attached to an university which serves two complementary purposes to support the curricula, and to support the research of university organizations and students."@en ;
                 
                 rdfs:isDefinedBy <http://lod.tuwien.ac.at/organization/vocab#> .



###  http://lod.tuwien.ac.at/organization/vocab#Center

:Center rdf:type owl:Class ;
        
        rdfs:label "Zentrum"@de ,
                   "Center"@en ;
        
        owl:equivalentClass aiiso:Center ;
        
        rdfs:subClassOf :UniversityOrganizationalUnit ;
        
        owl:disjointWith :Department ,
                         :Faculty ,
                         :Institute ,
                         :ResearchGroup ;
        
        rdfs:comment "A Center is a group of people recognised by an organization as forming a cohesive group referred to by the organization as a center."@en ;
        
        rdfs:isDefinedBy <http://lod.tuwien.ac.at/organization/vocab#> .



###  http://lod.tuwien.ac.at/organization/vocab#Deanery

:Deanery rdf:type owl:Class ;
         
         rdfs:label "Dekanat"@de ,
                    "Deanery"@en ;
         
         rdfs:subClassOf :UniversityOrganizationalUnit ;
         
         owl:disjointWith :Department ,
                          :Faculty ,
                          :Institute ,
                          :ResearchGroup ;
         
         rdfs:comment "A deanery is a organizational unit inside of an university, which administrates a faculty or a department."@en ;
         
         rdfs:isDefinedBy <http://lod.tuwien.ac.at/organization/vocab#> .



###  http://lod.tuwien.ac.at/organization/vocab#Department

:Department rdf:type owl:Class ;
            
            rdfs:label "Abteilung"@de ,
                       "Department"@en ;
            
            owl:equivalentClass aiiso:Department ;
            
            rdfs:subClassOf :UniversityOrganizationalUnit ;
            
            owl:disjointWith :Faculty ,
                             :Institute ,
                             :ResearchGroup ;
            
            rdfs:comment "A Department is a group of people recognised by an organization as forming a cohesive group referred to by the organization as a department."@en ;
            
            rdfs:isDefinedBy <http://lod.tuwien.ac.at/organization/vocab#> .



###  http://lod.tuwien.ac.at/organization/vocab#EducationRole

:EducationRole rdf:type owl:Class ;
               
               rdfs:subClassOf :EmploymentRole ;
               
               skos:altLabel "Ausbildende"@de ;
               
               skos:prefLabel "Ausbildender"@de ;
               
               rdfs:comment "DIese Rolle inkludiert die Ausbildung und Unterstützung in Bezug auf Ausbildung und Vorbereitung."@de ;
               
               skos:prefLabel "Educator"@en ;
               
               rdfs:comment "This role includes education or supporting function in regard of education and preperation."@en ;
               
               rdfs:isDefinedBy <http://lod.tuwien.ac.at/organization/vocab#> .



###  http://lod.tuwien.ac.at/organization/vocab#Employment

:Employment rdf:type owl:Class ;
            
            rdfs:label "Anstellung"@de ,
                       "Employment"@en ;
            
            rdfs:subClassOf :UniversityMembership ;
            
            rdfs:comment "Beschreibt die Anstellung eines Agenten in einer Universitätsorganisationen. Repräsentiert eine n-dimensionale Beziehung zwischen einem Agenten, einer Universitätsorganisation und einer Anstellungsrolle (z.B.: Tutor, Dozent, ...)."@de ,
                         "Indicates the employment of an Agent in an university organization. Represents an n-ary relation between an Agent, an University Organization and an Employment Role (e.g. tutor, docent, ...)."@en ;
            
            rdfs:isDefinedBy <http://lod.tuwien.ac.at/organization/vocab#> .



###  http://lod.tuwien.ac.at/organization/vocab#EmploymentRole

:EmploymentRole rdf:type owl:Class ;
                
                rdfs:subClassOf :UniversityRole ;
                
                skos:altLabel "Angestellte"@de ;
                
                skos:prefLabel "Angestellter"@de ,
                               "Employee"@en ;
                
                rdfs:isDefinedBy <http://lod.tuwien.ac.at/organization/vocab#> .



###  http://lod.tuwien.ac.at/organization/vocab#Faculty

:Faculty rdf:type owl:Class ;
         
         rdfs:label "Fakultät"@de ,
                    "Faculty"@en ;
         
         owl:equivalentClass aiiso:Faculty ;
         
         rdfs:subClassOf :UniversityOrganizationalUnit ;
         
         owl:disjointWith :Institute ,
                          :ResearchGroup ;
         
         rdfs:comment "A Faculty is a group of people recognised by an organization as forming a cohesive group referred to by the organization as a faculty."@en ;
         
         rdfs:isDefinedBy <http://lod.tuwien.ac.at/organization/vocab#> .



###  http://lod.tuwien.ac.at/organization/vocab#Institute

:Institute rdf:type owl:Class ;
           
           rdfs:label "Institut"@de ,
                      "Institute"@en ;
           
           owl:equivalentClass aiiso:Institute ;
           
           rdfs:subClassOf :UniversityOrganizationalUnit ;
           
           owl:disjointWith :ResearchGroup ;
           
           rdfs:comment "An Institute is a group of people recognised by an organization as forming a cohesive group referred to by the organization as an institute."@en ;
           
           rdfs:isDefinedBy <http://lod.tuwien.ac.at/organization/vocab#> .



###  http://lod.tuwien.ac.at/organization/vocab#ResearchCenter

:ResearchCenter rdf:type owl:Class ;
                
                rdfs:label "Forschungszentrum"@de ,
                           "Research center"@en ,
                           <http://lod.tuwien.ac.at/organization/vocab#> ;
                
                rdfs:subClassOf :Center ;
                
                rdfs:comment "A Center is a group of people recognised by an organization as forming a cohesive group referred to by the organization as a research center."@en .



###  http://lod.tuwien.ac.at/organization/vocab#ResearchGroup

:ResearchGroup rdf:type owl:Class ;
               
               rdfs:label "Forschungsgruppe"@de ,
                          "Research group"@en ;
               
               owl:equivalentClass aiiso:ResearchGroup ;
               
               rdfs:subClassOf :UniversityOrganizationalUnit ;
               
               rdfs:comment "A Research Group is a group of people recognised by an organization as forming a cohesive group referred to by the organization as a research group."@en ;
               
               rdfs:isDefinedBy <http://lod.tuwien.ac.at/organization/vocab#> .



###  http://lod.tuwien.ac.at/organization/vocab#StudentRole

:StudentRole rdf:type owl:Class ;
             
             rdfs:subClassOf :UniversityRole ;
             
             skos:prefLabel "Student"@de ;
             
             skos:altLabel "Studentin"@de ,
                           "Studierende"@de ,
                           "Studierender"@de ;
             
             skos:prefLabel "Student"@en ;
             
             rdfs:isDefinedBy <http://lod.tuwien.ac.at/organization/vocab#> .



###  http://lod.tuwien.ac.at/organization/vocab#TutorRole

:TutorRole rdf:type owl:Class ;
           
           rdfs:subClassOf :EducationRole ;
           
           skos:prefLabel "Tutor"@de ;
           
           skos:altLabel "Tutorin"@de ;
           
           skos:prefLabel "Tutor"@en ;
           
           rdfs:isDefinedBy <http://lod.tuwien.ac.at/organization/vocab#> .



###  http://lod.tuwien.ac.at/organization/vocab#University

:University rdf:type owl:Class ;
            
            rdfs:label "Universität"@de ,
                       "University"@en ;
            
            rdfs:subClassOf :UniversityOrganization ,
                            org:FormalOrganization ;
            
            rdfs:comment "Eine Institution höherer Ausbildung und Forschung, welche akademische Grade in verschieden Fachbereichen verleiht und ein grundständiges Studium beziehungsweise postgraduelle Ausbildung ermöglicht."@de ,
                         "An institution of higher education and research, which grants academic degrees in a variety of subjects, and provides both undergraduate education and postgraduate education."@en ;
            
            rdfs:isDefinedBy <http://lod.tuwien.ac.at/organization/vocab#> .



###  http://lod.tuwien.ac.at/organization/vocab#UniversityMembership

:UniversityMembership rdf:type owl:Class ;
                      
                      rdfs:label "Universitätsmitgliedschaft"@de ,
                                 "University membership"@en ,
                                 <http://lod.tuwien.ac.at/organization/vocab#> ;
                      
                      rdfs:subClassOf org:Membership ;
                      
                      rdfs:comment "Beschreibt die Natur der Mitgliedschaft eines Agenten in einer Universitätsorganisation. Die Klasse repräsentiert eine n-dimensionale Beziehung zwischen einem Agenten, einer Universitätsorganisation und der Universitätsrolle (z.B. Student, Vortragender, ...)."@de ,
                                   "Indicates the nature of an Agent's membership of an university organization. Represents an n-ary relation between an Agent, an University Organization and a University Role (e.g. Student, Lecturer,...)."@en .



###  http://lod.tuwien.ac.at/organization/vocab#UniversityOrganization

:UniversityOrganization rdf:type owl:Class ;
                        
                        rdfs:label "Universitätsorganisation"@de ,
                                   "University organization"@en ;
                        
                        rdfs:subClassOf org:Organization ;
                        
                        rdfs:comment "Beschreibt eine Organisation, die einer Universität zugeordnet werden kann oder selbst eine Universität ist."@de ,
                                     "Describes an organization, which can be assigned to an university or is an university itself."@en ;
                        
                        rdfs:isDefinedBy <http://lod.tuwien.ac.at/organization/vocab#> .



###  http://lod.tuwien.ac.at/organization/vocab#UniversityOrganizationalUnit

:UniversityOrganizationalUnit rdf:type owl:Class ;
                              
                              rdfs:label "Organisationseinheit einer Universität"@de ,
                                         "University organization unit"@en ;
                              
                              rdfs:subClassOf :UniversityOrganization ,
                                              org:OrganizationalUnit ;
                              
                              rdfs:comment "Beschreibt die Organisationseinehit einer Universität."@de ,
                                           "Describes the organizational unit of an university."@en ;
                              
                              rdfs:isDefinedBy <http://lod.tuwien.ac.at/organization/vocab#> .



###  http://lod.tuwien.ac.at/organization/vocab#UniversityRole

:UniversityRole rdf:type owl:Class ;
                
                rdfs:label "Universitätsrolle"@de ,
                           "University role"@en ;
                
                rdfs:subClassOf org:Role ;
                
                rdfs:comment "Beschreibt eine Rolle innerhalb der Universität. Zum Beispiel die Rolle eines Studenten oder Vorlesenden."@de ,
                             "Describes a role inside of an university. E.g. student or lecturer."@de ;
                
                rdfs:isDefinedBy <http://lod.tuwien.ac.at/organization/vocab#> .



###  http://purl.org/vocab/aiiso/schema#Center

aiiso:Center rdf:type owl:Class .



###  http://purl.org/vocab/aiiso/schema#Department

aiiso:Department rdf:type owl:Class .



###  http://purl.org/vocab/aiiso/schema#Faculty

aiiso:Faculty rdf:type owl:Class .



###  http://purl.org/vocab/aiiso/schema#Institute

aiiso:Institute rdf:type owl:Class .



###  http://purl.org/vocab/aiiso/schema#ResearchGroup

aiiso:ResearchGroup rdf:type owl:Class .



###  http://xmlns.com/foaf/0.1/Person

foaf:Person rdf:type owl:Class ;
            
            rdfs:isDefinedBy foaf: .





#################################################################
#
#    Individuals
#
#################################################################


###  http://lod.tuwien.ac.at/person/contributor/Kevin_Haller

<http://lod.tuwien.ac.at/person/contributor/Kevin_Haller> rdf:type owl:NamedIndividual ,
                                                                   foaf:Person .




###  Generated by the OWL API (version 3.5.1) http://owlapi.sourceforge.net

